wip: add a proof of bn_from_bytes_be_lemma

code/experimental/rsapss/Hacl.Spec.Bignum.Convert.fst
@@ -51,11 +51,110 @@ let bn_to_bytes_be len b =
 
 ///
 ///  Lemmas
-/// 
+///
+
+val reverse: #len:size_nat -> b:lseq uint64 len -> lseq uint64 len
+let reverse #len b = createi len (fun i -> b.[len - i - 1])
+
+val twice_reverse: #len:size_nat -> b:lseq uint64 len -> Lemma (reverse (reverse b) == b)
+let twice_reverse #len b =
+  let lemma_aux (i:nat{i < len}) : Lemma ((reverse (reverse b)).[i] == b.[i]) = () in
+  Classical.forall_intro lemma_aux;
+  eq_intro (reverse (reverse b)) b
+
+val reverse_slice1: #len:size_pos -> b:lseq uint64 len -> Lemma
+  (slice (reverse b) 1 len == reverse (slice b 0 (len - 1)))
+let reverse_slice1 #len b =
+  let lemma_aux (i:nat{i < len - 1}) : Lemma ((slice (reverse b) 1 len).[i] == (reverse (slice b 0 (len - 1))).[i]) =
+    () in
+  Classical.forall_intro lemma_aux;
+  eq_intro (slice (reverse b) 1 len) (reverse (slice b 0 (len - 1)))
+
+
+val bn_from_bytes_be_is_uints_from_bytes_be_reverse: len:size_nat{8 * len <= max_size_t} -> b:lseq uint8 (8 * len) -> Lemma
+  (bn_from_bytes_be_ len b == reverse (uints_from_bytes_be b))
+let bn_from_bytes_be_is_uints_from_bytes_be_reverse len b =
+  let lemma_aux (i:nat{i < len}) : Lemma ((bn_from_bytes_be_ len b).[i] == (reverse #len (uints_from_bytes_be b)).[i]) =
+    index_uints_from_bytes_be #U64 #SEC #len b (len - i - 1) in
+  Classical.forall_intro lemma_aux;
+  eq_intro (bn_from_bytes_be_ len b) (reverse (uints_from_bytes_be b))
+
+
+val bn_v_is_nat_from_intseq_le_lemma: len:size_nat -> b:lseq uint64 len -> Lemma (bn_v b == nat_from_intseq_be (reverse b))
+let rec bn_v_is_nat_from_intseq_le_lemma len b =
+  if len = 0 then bn_eval0 b
+  else begin
+    let b1 = slice b 0 (len - 1) in
+    bn_v_is_nat_from_intseq_le_lemma (len - 1) b1;
+    assert (bn_v b1 == nat_from_intseq_be (reverse b1));
+
+    bn_eval_split_i #len b (len - 1);
+    //assert (bn_v b == bn_v b1 + pow2 (64 * (len - 1)) * bn_v (slice b (len - 1) len));
+    bn_eval_unfold_i #1 (slice b (len - 1) len) 1;
+    bn_eval0 #1 (slice b (len - 1) len);
+    assert (bn_v (slice b (len - 1) len) == v b.[len - 1]);
+    assert (bn_v b == nat_from_intseq_be (reverse b1) + pow2 (64 * (len - 1)) * v b.[len - 1]);
+
+    nat_from_intseq_be_slice_lemma (reverse b) 1;
+    //assert (nat_from_intseq_be (reverse b) == nat_from_intseq_be (slice (reverse b) 1 len) + pow2 ((len - 1) * 64) * nat_from_intseq_be (slice (reverse b) 0 1));
+    reverse_slice1 #len b;
+    //assert (slice (reverse b) 1 len == reverse (slice b 0 (len - 1)));
+    //assert (nat_from_intseq_be (reverse b) == nat_from_intseq_be (reverse b1) + pow2 ((len - 1) * 64) * nat_from_intseq_be (slice (reverse b) 0 1));
+    assert ((reverse b).[0] == b.[len - 1]);
+    nat_from_intseq_be_lemma0 (slice (reverse b) 0 1);
+    assert (nat_from_intseq_be (slice (reverse b) 0 1) == v b.[len - 1]);
+    assert  (bn_v b == nat_from_intseq_be (reverse b));
+    () end
+
+
+val bn_from_bytes_be_lemma_: len:size_nat{8 * len <= max_size_t} -> b:lseq uint8 (8 * len) -> Lemma
+  (bn_v (bn_from_bytes_be_ len b) == nat_from_bytes_be b)
+let bn_from_bytes_be_lemma_ len b =
+  bn_v_is_nat_from_intseq_le_lemma len (bn_from_bytes_be_ len b);
+  bn_from_bytes_be_is_uints_from_bytes_be_reverse len b;
+  twice_reverse (uints_from_bytes_be #U64 #SEC #len b);
+  assert (bn_v (bn_from_bytes_be_ len b) == nat_from_intseq_be (uints_from_bytes_be #U64 #SEC #len b));
+  assume (nat_from_intseq_be (uints_from_bytes_be #U64 #SEC #len b) == nat_from_bytes_be b)
+  //the uints_from_bytes_be_nat_lemma b lemma from master
+
+val lemma_nat_from_bytes_be_zeroes: len:size_nat -> b:lseq uint8 len -> Lemma
+  (requires (forall (i:nat). i < len ==> b.[i] == u8 0))
+  (ensures  nat_from_intseq_be b == 0)
+
+let rec lemma_nat_from_bytes_be_zeroes len b =
+  if len = 0 then ()
+  else begin
+    nat_from_intseq_be_slice_lemma #U8 #SEC #len b 1;
+    nat_from_intseq_be_lemma0 (slice b 0 1);
+    lemma_nat_from_bytes_be_zeroes (len-1) (slice b 1 len) end
+
+
+val nat_from_bytes_be_eq_lemma: len0:size_nat -> len:size_nat{len0 <= len} -> b:lseq uint8 len0 -> Lemma
+ (let tmp = create len (u8 0) in
+  nat_from_intseq_be b == nat_from_intseq_be (update_sub tmp (len - len0) len0 b))
+
+let nat_from_bytes_be_eq_lemma len0 len b =
+  let tmp = create len (u8 0) in
+  let r = update_sub tmp (len - len0) len0 b in
+  assert (slice r (len - len0) len == b);
+  assert (forall (i:nat). i < len - len0 ==> r.[i] == u8 0);
+  nat_from_intseq_be_slice_lemma #U8 #SEC #len r (len - len0);
+  assert (nat_from_intseq_be r == nat_from_intseq_be (slice r (len - len0) len) + pow2 (len0 * 8) * nat_from_intseq_be (Seq.slice r 0 (len - len0)));
+  assert (nat_from_intseq_be r == nat_from_intseq_be b + pow2 (len0 * 8) * nat_from_intseq_be (Seq.slice r 0 (len - len0)));
+  lemma_nat_from_bytes_be_zeroes (len - len0) (Seq.slice r 0 (len - len0))
+
 
 val bn_from_bytes_be_lemma: len:size_pos{8 * blocks len 8 <= max_size_t} -> b:lseq uint8 len -> Lemma
   (bn_v (bn_from_bytes_be len b) == nat_from_bytes_be b)
-let bn_from_bytes_be_lemma len b = admit()
+let bn_from_bytes_be_lemma len b =
+  let bnLen = blocks len 8 in
+  let tmpLen = 8 * bnLen in
+  let tmp = create tmpLen (u8 0) in
+  let tmp = update_sub tmp (tmpLen - len) len b in
+  let res = bn_from_bytes_be_ bnLen tmp in
+  bn_from_bytes_be_lemma_ bnLen tmp;
+  assert (bn_v (bn_from_bytes_be_ bnLen tmp) == nat_from_bytes_be tmp);
+  nat_from_bytes_be_eq_lemma len tmpLen b
 
 
 val bn_to_bytes_be_lemma: len:size_pos{8 * blocks len 8 <= max_size_t} -> b:lbignum (blocks len 8){bn_v b < pow2 (8 * len)} -> Lemma
